examples/elliptic/arm/instructionScript.sml
@@ -150,60 +150,33 @@ val options_encode2_def = Define`
     word_modify (\i b. (i = 24) /\ opt.Pre \/ (i = 23) /\ opt.Up \/
                        (i = 21) /\ opt.Wb \/ (i = 5) /\ h) (0w:word32)`;
 
+val data_proc_encode_def = Define`
+  data_proc_encode cond (op:word4) s (Rn:word4) (Rd:word4) Op2 =
+    condition_encode cond !! w2w op << 21 !! (s => 0x100000w | 0w) !!
+       w2w Rn << 16 !! w2w Rd << 12 !! addr_mode1_encode Op2`;
+
 val instruction_encode_def = Define`
   instruction_encode i =
     case i of
        B  cond offset24 -> condition_encode cond !! 0xA000000w !! w2w offset24
     || BL cond offset24 -> condition_encode cond !! 0xB000000w !! w2w offset24
     || SWI cond -> condition_encode cond !! 0xF000000w
-    || AND cond s Rd Rn Op2 ->
-         condition_encode cond !! (s => 0x100000w | 0w) !!
-         w2w Rn << 16 !! w2w Rd << 12 !! addr_mode1_encode Op2
-    || EOR cond s Rd Rn Op2 ->
-         condition_encode cond !! (s => 0x300000w | 0x200000w) !!
-         w2w Rn << 16 !! w2w Rd << 12 !! addr_mode1_encode Op2
-    || SUB cond s Rd Rn Op2 ->
-         condition_encode cond !! (s => 0x500000w | 0x400000w) !!
-         w2w Rn << 16 !! w2w Rd << 12 !! addr_mode1_encode Op2
-    || RSB cond s Rd Rn Op2 ->
-         condition_encode cond !! (s => 0x700000w | 0x600000w) !!
-         w2w Rn << 16 !! w2w Rd << 12 !! addr_mode1_encode Op2
-    || ADD cond s Rd Rn Op2 ->
-         condition_encode cond !! (s => 0x900000w | 0x800000w) !!
-         w2w Rn << 16 !! w2w Rd << 12 !! addr_mode1_encode Op2
-    || ADC cond s Rd Rn Op2 ->
-         condition_encode cond !! (s => 0xB00000w | 0xA00000w) !!
-         w2w Rn << 16 !! w2w Rd << 12 !! addr_mode1_encode Op2
-    || SBC cond s Rd Rn Op2 ->
-         condition_encode cond !! (s => 0xD00000w | 0xC00000w) !!
-         w2w Rn << 16 !! w2w Rd << 12 !! addr_mode1_encode Op2
-    || RSC cond s Rd Rn Op2 ->
-         condition_encode cond !! (s => 0xF00000w | 0xE00000w) !!
-         w2w Rn << 16 !! w2w Rd << 12 !! addr_mode1_encode Op2
-    || TST cond Rn Op2 ->
-         condition_encode cond !! 0x1100000w !!
-         w2w Rn << 16 !! addr_mode1_encode Op2
-    || TEQ cond Rn Op2 ->
-         condition_encode cond !! 0x1300000w !!
-         w2w Rn << 16 !! addr_mode1_encode Op2
-    || CMP cond Rn Op2 ->
-         condition_encode cond !! 0x1500000w !!
-         w2w Rn << 16 !! addr_mode1_encode Op2
-    || CMN cond Rn Op2 ->
-         condition_encode cond !! 0x1700000w !!
-         w2w Rn << 16 !! addr_mode1_encode Op2
-    || ORR cond s Rd Rn Op2 ->
-         condition_encode cond !! (s => 0x1900000w | 0x1800000w) !!
-         w2w Rn << 16 !! w2w Rd << 12 !! addr_mode1_encode Op2
-    || MOV cond s Rd Op2 ->
-         condition_encode cond !! (s => 0x1B00000w | 0x1A00000w) !!
-         w2w Rd << 12 !! addr_mode1_encode Op2
-    || BIC cond s Rd Rn Op2 ->
-         condition_encode cond !! (s => 0x1D00000w | 0x1C00000w) !!
-         w2w Rn << 16 !! w2w Rd << 12 !! addr_mode1_encode Op2
-    || MVN cond s Rd Op2 ->
-         condition_encode cond !! (s => 0x1F00000w | 0x1E00000w) !!
-         w2w Rd << 12 !! addr_mode1_encode Op2
+    || AND cond s Rd Rn Op2 -> data_proc_encode cond 0w s Rn Rd Op2
+    || EOR cond s Rd Rn Op2 -> data_proc_encode cond 1w s Rn Rd Op2
+    || SUB cond s Rd Rn Op2 -> data_proc_encode cond 2w s Rn Rd Op2
+    || RSB cond s Rd Rn Op2 -> data_proc_encode cond 3w s Rn Rd Op2
+    || ADD cond s Rd Rn Op2 -> data_proc_encode cond 4w s Rn Rd Op2
+    || ADC cond s Rd Rn Op2 -> data_proc_encode cond 5w s Rn Rd Op2
+    || SBC cond s Rd Rn Op2 -> data_proc_encode cond 6w s Rn Rd Op2
+    || RSC cond s Rd Rn Op2 -> data_proc_encode cond 7w s Rn Rd Op2
+    || TST cond Rn Op2      -> data_proc_encode cond 8w T Rn 0w Op2
+    || TEQ cond Rn Op2      -> data_proc_encode cond 9w T Rn 0w Op2
+    || CMP cond Rn Op2      -> data_proc_encode cond 10w T Rn 0w Op2
+    || CMN cond Rn Op2      -> data_proc_encode cond 11w T Rn 0w Op2
+    || ORR cond s Rd Rn Op2 -> data_proc_encode cond 12w s Rn Rd Op2
+    || MOV cond s Rd Op2    -> data_proc_encode cond 13w s 0w Rd Op2
+    || BIC cond s Rd Rn Op2 -> data_proc_encode cond 14w s Rn Rd Op2
+    || MVN cond s Rd Op2    -> data_proc_encode cond 15w s 0w Rd Op2
     || MUL cond s Rd Rm Rs ->
          condition_encode cond !! (s => 0x100090w | 0x90w) !!
          w2w Rd << 16 !! w2w Rs << 8 !! w2w Rm
